
\documentclass[11pt]{amsart}
\usepackage[usenames,dvipsnames,condensed]{xcolor}
%\usepackage[a4paper,right=.7in,left=.7in,top=.6in,bottom=.5in]{geometry}
\usepackage{fullpage}
\usepackage{amsmath}
\usepackage{mathtools}
\usepackage{amsthm}
\usepackage{amsfonts}
\usepackage[UKenglish]{babel}
\usepackage{graphicx}
\usepackage{cite}
\usepackage{multicol}
\usepackage{multirow}
\usepackage{afterpage}
\usepackage{sansmath}
\usepackage{marginnote}
\usepackage[version=3]{mhchem}

\usepackage{boxedminipage}
%\usepackage{titlesec}

\usepackage{hyperref}
\hypersetup{
    backref =       true,
    pagebackref  =  true,
    colorlinks =    true,
    linkcolor =     purple,
    anchorcolor =   [rgb]{0.0,0.0,0.0},
    citecolor =     [rgb]{0.0,0.0,0.0},
    filecolor =     [rgb]{0.0,0.0,0.0},
    urlcolor =      [rgb]{0.0,0.0,0.0},
    pdftitle=       {Title},
    pdfsubject=     {Title},
    pdfauthor=      {K. Sasaki}
}
 
%\reversemarginpar

\setcounter{tocdepth}{4}
\setcounter{secnumdepth}{4}

%\titleformat{\paragraph}
%{\normalfont\normalsize\bfseries}{\theparagraph}{1em}{}
%\titlespacing*{\paragraph}
%{0pt}{3.25ex plus 1ex minus .2ex}{1.5ex plus .2ex}



%\usepackage{fancyhdr}
%\pagestyle{fancy}
%\lhead{Predoc/EMBO CBB courses, script}
%\rhead{Karin Sasaki}

%------------------------------------------------------------------------------------------------------------%


\begin{document}

\[\frac{dA}{dt} = -k_{1}*A\]

\[\frac{dA}{dt} = -k_{2f}*A + k_{2r}*B\]
\[\frac{dB}{dt} = k_{2f}*A - k_{2r}*B\]

Karin's
\[Ssk2 + ATP \xrightarrow[]{k_1^{MAP}} SskP + ADP \]
\[Ssk2P \xrightarrow[]{k_{-1}^{MAP}} Ssk2 \]
\[Ssk2P + Pbs2 \xrightarrow[]{k_2^{MAP}} Ssk2 + Pbs2P\]
\[Pbs2P \xrightarrow[]{k_{-2}^{MAP}} Pbs2\]
\[Ssk2P + Pbs2P \xrightarrow[]{k_3^{MAP}} Ssk2 + Pbs2P_2\]
\[Pbs2P_2 \xrightarrow[]{k_{-3}^{MAP}} Pbs2P\]
\[Hog1 + Pbs2P_2 \xrightarrow[]{k_4^{MAP}} Hog1P + Pbs2P\]
\[Hog1P \xrightarrow[]{k_v{-4}^{MAP}} Hog1\]
\[Hog1P + Pbs2P_2 \xrightarrow[]{k_5^{MAP}} Hog1P_{2cyt} + Pbs2P\]
\[Hog1P_{2cyt} \xrightarrow[]{k_{-5}^{MAP}} Hog1P\]
\[Hog1P_{2cyt} \xrightarrow[]{k_{trans}} Hog1P_{2nuc}\]
\[Hog1P_{2nuc} \xrightarrow[]{k_{dephos}} Hog1_{nuc}\]
\[Hog1_{nuc} \xrightarrow[]{k_{trans1}} Hog1\]
\[Hog1 \xrightarrow[]{k_{trans2}} Hog1_{nuc}\]

\clearpage
Paper's
\[Ssk2 + ATP \xrightarrow[]{k_1^{MAP}} SskP + ADP \]
\[Ssk2P \xrightarrow[]{k_{-1}^{MAP}} Ssk2 \]
\[Pbs2 + ATP \xrightarrow[]{k_2^{MAP}} ADP + Pbs2P\]
\[Pbs2P \xrightarrow[]{k_{-2}^{MAP}} Pbs2\]
\[Pbs2P + ATP \xrightarrow[]{k_3^{MAP}} Pbs2P_2 + ADP\]
\[Pbs2P_2 \xrightarrow[]{k_{-3}^{MAP}} Pbs2P\]
\[Hog1 + ATP \xrightarrow[]{k_4^{MAP}} Hog1P + ADP\]
\[Hog1P \xrightarrow[]{k_v{-4}^{MAP}} Hog1\]
\[Hog1P + ATP \xrightarrow[]{k_5^{MAP}} Hog1P_{2cyt} + ADP\]
\[Hog1P_{2cyt} \xrightarrow[]{k_{-5}^{MAP}} Hog1P\]
\[Hog1P_{2cyt} \xrightarrow[]{k_{trans}} Hog1P_{2nuc}\]
\[Hog1P_{2nuc} \xrightarrow[]{k_{dephos}} Hog1_{nuc}\]
\[Hog1_{nuc} \xrightarrow[]{k_{trans1}} Hog1\]
\[Hog1 \xrightarrow[]{k_{trans2}} Hog1_{nuc}\]

\[v_1^{MAP} = k_1^{MAP}*Ssk2*Ssk1\]
\[v_{-1}^{MAP} =k_{-1}^{MAP}*Ssk2P \]
\[v_2^{MAP} = k_2^{MAP}*Ssk2*Pbs2\]
\[v_{-2}^{MAP} = k_{-2}*Pbs2P\]
\[v_3^{MAP} = k_3^{MAP}*Ssk2P*Pbs2P\]
\[v_{-3}^{MAP} = k_{-3}*Pbs2P_2\]
\[v_4^{MAP} = k_4^{MAP}*Hog1*PbsP_2\]
\[v_{-4}^{MAP} = k_{-4}*Hog1P\]
\[v_{5}^{MAP} = k_5*Hog1P*Pbs2P_2\]
\[v_{-5}^{MAP} = k_{-5}*Hog1P_{2cyt}\]
\[v_{trans} = k_{trans}*Hog1P_{2cyt}\]
\[v_{dephos} = k_{dephos}*Hog1P_{2nuc}*Ptp2\]
\[v_{trans1} = k_{trans1}*Hog1_{nuc}\]
\[v_{trans2} = k_{trans2}*Hog1\]

\clearpage
Karin's 

\[\frac{dSsk2}{dt} = -v_1^{MAP} + v_{-1}^{MAP} + v_2^{MAP} + v_3^{MAP}\]
\[\frac{dSsk2P}{dt} = v_1^{MAP} - v_{-1}^{MAP} - v_2^{MAP} - v_{3}^{MAP}\]
\[\frac{dPbs2}{dt} = -v_2^{MAP} + v_{-2}^{MAP}\]
\[\frac{dPbs2P}{dt} = v_2^{MAP} - v_{-2}^{MAP}- v_3^{MAP} + v_{-3}^{MAP} + v_4^{MAP}\]
\[\frac{dPbs2P_2}{dt} = v_3^{MAP} - v_{-3}^{MAP} - v_4^{MAP} - v_5^{MAP}\]
\[\frac{dHog1}{dt} = -v_4^{MAP} + v_{-4}^{MAP} + v_{trans1} - v_{trans2}\]
\[\frac{dHog1P}{dt} = v_4^{MAP} - v_{-4}^{MAP} - v_{5}^{MAP} + v_{-5}^{MAP} \]
\[\frac{dHog1P_{2cyt}}{dt} =  v_{5}^{MAP} - v_{-5}^{MAP} - v_{trans}\]
\[\frac{dHog1P_{2nuc}}{dt} = v_{trans} - v_{dephos}\]
\[\frac{dHog1_{nuc}}{dt} = -v_{trans1} + v_{dephos} + v_{trans2} \]

Paper
\[\frac{dSsk2}{dt} = -v_1^{MAP} + v_{-1}^{MAP} \]
\[\frac{dSsk2P}{dt} = v_1^{MAP} - v_{-1}^{MAP} \]
\[\frac{dPbs2}{dt} = -v_2^{MAP} + v_{-2}^{MAP}\]
\[\frac{dPbs2P}{dt} = v_2^{MAP} - v_{-2}^{MAP} - v_3^{MAP} + v_{-3}^{MAP}\]
\[\frac{dPbs2P_2}{dt} = v_3^{MAP} - v_{-3}^{MAP} \]
\[\frac{dHog1}{dt} = -v_4^{MAP} + v_{-4}^{MAP} + v_{trans1} - v_{trans2}\]
\[\frac{dHog1P}{dt} = v_4^{MAP} - v_{-4}^{MAP} - v_{5}^{MAP} + v_{-5}^{MAP} \]
\[\frac{dHog1P_{2cyt}}{dt} =  v_{5}^{MAP} - v_{-5}^{MAP} - v_{trans}\]
\[\frac{dHog1P_{2nuc}}{dt} = v_{trans} - v_{dephos}\]
\[\frac{dHog1_{nuc}}{dt} = -v_{trans1} + v_{dephos} + v_{trans2} \]


\clearpage

\begin{align}
\cee{Sln1 &->[k_1^{TCS}]Sln1P} \\
\cee{Sln1P + Ypd1 &<=>[k_{2}^{TCS}][k_{-2}^{TCS}] Sln1 + Ypd1P} \\
\cee{Ypd1P + Ssk1 &->[k_3^{TCS}] Ypd1 + Ssk1P} \\
\cee{Ssk1P &->[k_4^{TCS}] Ssk1}
\end{align}

\[\frac{dVolume}{dt} = -v_0^{TCS}\]
\[\frac{dSln1}{dt} = -v_1^{TCS} + v_2^{TCS}\]
\[\frac{dSln1P}{dt} = v_1^{TCS} - v_2^{TCS}\]
\[\frac{dYpd1}{dt} = -v_2^{TCS} + v_3^{TCS}\]
\[\frac{dYpd1P}{dt} = v_2^{TCS} - v_3^{TCS}\]
\[\frac{dSsk1}{dt} = -v_3^{TCS} + v_4^{TCS}\]
\[\frac{dSsk1P}{dt} = v_3^{TCS} - v_4^{TCS}\]

\[v_0^{TCS} = k_0^{TCS}*SSk1\]
\[v_1^{TCS} = k_1^{TCS}*Sln1\]
\[v_2^{TCS} = k_2^{TCS}*Sln1*Ypd1 - k_{-2}^{TCS}*Sln1*Ypd1P\]
\[v_3^{TCS} = k_3^{TCS}*Ssk1*Ypd1P\]
\[v_4^{TCS} = k_4^{TCS}*Ssk1P\]

\clearpage
\[v0 = k0*Receptor\]
\[v1 = k1*MAPKKK*Receptor\]
\[v2 = k2*MAPKKKP*Phosphotase\]
\[v3 = k3*MAPKK*MAPKKKP    \]
\[v4 = k4*MAPKKP*Phosphotase\]
\[v5 = k5*MAPK*MAPKKP    \]
\[v6 = k6*MAPKP*Phosphotase\]

\[\frac{dReceptor}{dt} = -v0\]
\[\frac{dMAPKKKP}{dt} = v1 - v2\]
\[\frac{dMAPKKP}{dt} = v3 - v4\]
\[\frac{dMAPKP}{dt} = v5 - v6\]
\[\frac{dMAPKKK}{dt} = -dMAPKKKP\]
\[\frac{dMAPKK}{dt} = -dMAPKKP\]
\[\frac{dMAPK}{dt} = -dMAPKP   \]
\[\frac{dPhosphotase}{dt} = 0\]



\clearpage
\[v_0 = k_0*Ssk1\]
\[v_1^{MAP} = k_1^{MAP}*Ssk2*Ssk1\]
\[v_{-1}^{MAP} =k_{-1}^{MAP}*Ssk2P \]
\[v_2^{MAP} = k_2^{MAP}*Ssk2*Pbs2\]
\[v_{-2}^{MAP} = k_{-2}*Pbs2P\]
\[v_3^{MAP} = k_3^{MAP}*Ssk2P*Pbs2P\]
\[v_{-3}^{MAP} = k_{-3}*Pbs2P_2\]
\[v_4^{MAP} = k_4^{MAP}*Hog1*PbsP_2\]
\[v_{-4}^{MAP} = k_{-4}*Hog1P\]
\[v_{5}^{MAP} = k_5*Hog1P*Pbs2P_2\]
\[v_{-5}^{MAP} = k_{-5}*Hog1P_2\]

\[\frac{dSsk1}{dt} = -v_0^{MAP}\]
\[\frac{dSsk2}{dt} = -v_1^{MAP} + v_{-1}^{MAP} \]
\[\frac{dSsk2P}{dt} = v_1^{MAP} - v_{-1}^{MAP} \]
\[\frac{dPbs2}{dt} = -v_2^{MAP} + v_{-2}^{MAP}\]
\[\frac{dPbs2P}{dt} = v_2^{MAP} - v_{-2}^{MAP} - v_3^{MAP} + v_{-3}^{MAP}\]
\[\frac{dPbs2P_2}{dt} = v_3^{MAP} - v_{-3}^{MAP} \]
\[\frac{dHog1}{dt} = -v_4^{MAP} + v_{-4}^{MAP}\]
\[\frac{dHog1P}{dt} = v_4^{MAP} - v_{-4}^{MAP} - v_{5}^{MAP} + v_{-5}^{MAP} \]
\[\frac{dHog1P_2}{dt} =  v_{5}^{MAP} - v_{-5}^{MAP}\]

\clearpage

\[vts = kts_1*Hog_1P_{2nuc}\]
\[vex = kex*mRNA_{nuc}\]
\[vrd = kts*mRNA_{cyt}\]
\[vtl = ktl*mRNA_{cyt}\]
\[vpd = kpd*Protein\]


\[\frac{dmRNA_{nuc}}{dt} = vts - vex\]
\[\frac{dmRNA_{cyt}}{dt} = vex - vrd\]
\[\frac{dProtein}{dt} = vtl - vpd\]

\[f(E, S, ES)\]


\clearpage

\[[H2](t), [O2](t), [H2O](t), [C](t), [CO2](t)\]

\

\

\[
y(t) = 
\begin{pmatrix}
[H_2](t) \\
[O_2](t) \\
[H_2O](t) \\
[C](t) \\
[CO_2](t) 
\end{pmatrix}
 \]

\

\ 

 
\[{\dot  {y}}\equiv {\frac  {dy}{dt}}=\left({\begin{array}{c}{\frac  {d[H_2]}{dt}}\\[6pt]{\frac  {d[O_2]}{dt}}\\[6pt]{\frac  {d[H_2O]}{dt}}\\[6pt]{\frac  {d[C]}{dt}}\\[6pt]{\frac  {d[CO_2]}{dt}}\\[6pt] \end{array}}\right)\]

\

\

\[\dot{y} = \Gamma V\]

\

\


\[{\dot  {y}}\equiv {\frac  {dy}{dt}}=\left({\begin{array}{c}{\frac  {d[H_2]}{dt}=  -k1*[H_2]^2*[O_2]}\\[6pt]{\frac  {d[O_2]}{dt} = -k1*[H_2]^2*[O_2] - k2*[C]*[O_2]}\\[6pt]{\frac  {d[H_2O]}{dt} =  2*k1*[H_2]^2*[O_2]}\\[6pt]{\frac  {d[C]}{dt} =  - k2*[C]*[O_2]}\\[6pt]{\frac  {d[CO_2]}{dt} =  k2*[C]*[O_2]}\\[6pt] \end{array}}\right)\]

\

\

\[
\Gamma = 
\begin{pmatrix}
 & H_2 & O_2 & H_2O & C & CO_2\\
R1: & -2 & -1 & 2 & 0 & 0\\
R2: & 0 & -1 & 0 & -1 & 1
\end{pmatrix}
 \]

\

\
 
 \[
\Gamma = 
\begin{pmatrix}
 & R1 & R2\\
H_2 &  -2 & 0\\
O_2 &  -1 & -1\\
H_2O &  2 & 0\\
C &  0 & -1\\
CO_2 &  0 & 1
\end{pmatrix}
 \]

\

\
 
\[
V = 
\begin{pmatrix}
k_1*[H_2]^2*[O_2]\\
k_2*[C]*[O_2]
\end{pmatrix}
 \]
 
 \[{\dot  {y}} 
 = \Gamma *V 
 =  \begin{pmatrix}
 & R1 & R2\\
H_2 &  -2 & 0\\
O_2 &  -1 & -1\\
H_2O &  2 & 0\\
C &  0 & -1\\
CO_2 &  0 & 1
\end{pmatrix} * 
\begin{pmatrix}
R1: & k1*[H_2]^2*[O_2]\\
R2: & k2*[C]*[O_2]
\end{pmatrix} 
=\left({\begin{array}{c}{\frac  {d[H_2]}{dt}=  -2*k1*[H_2]^2*[O_2]}\\[6pt]{\frac  {d[O_2]}{dt} = -k1*[H_2]^2*[O_2] - k2*[C]*[O_2]}\\[6pt]{\frac  {d[H_2O]}{dt} =  2*k1*[H_2]^2*[O_2]}\\[6pt]{\frac  {d[C]}{dt} =  - k2*[C]*[O_2]}\\[6pt]{\frac  {d[CO_2]}{dt} =  k2*[C]*[O_2]}\\[6pt] \end{array}}\right)\]


\

\

\[rate_{R1} = -\frac{1}{2}*\frac{d[H_2]}{dt}=-\frac{d[O_2]}{dt}=+\frac{1}{2}*\frac{d[H_2O]}{dt}\]

\

\

\[rate_{R1} = k_1[H_2]^2[O_2]\]

\

\

Enzymatic reaction

\[{\dot  {y}} 
 = \Gamma *V 
 =  \begin{pmatrix}
 & R1 & R2 & R3\\
S &  -1 & +1 & 0\\
E &  -1 & +1 & +1\\
SE &  +1 & -1 & -1\\
P &  0 & 0 & +1
\end{pmatrix} * 
\begin{pmatrix}
R1: & k_1*E*S\\
R2: & k_2*ES\\
R3: & k_3*ES
\end{pmatrix} 
=\left(
{\begin{array}{c}
{\frac  {dS}{dt}=  -k_1*E*S + k_2*ES}\\[6pt]
{\frac  {dE}{dt} = -k_1*E*S + (k_2+k_3)*ES}\\[6pt]
{\frac  {dES}{dt} =  k_1*E*S - (k_2+k_3)*ES}\\[6pt]
{\frac  {dP}{dt} = k_3*ES}\\[6pt] 
\end{array}}
\right)\]

\

\

Gene expression

\[{\dot  {y}} 
 = \Gamma *V 
 =  \begin{pmatrix}
 & R1 & R2 & R3 & R4\\
G & 0 & 0 & 0 & 0 \\
M & +1 & 0 & -1 & 0 \\
P &  0 & +1 & 0 & -1 \\ 
\end{pmatrix} * 
\begin{pmatrix}
R1: & k_1*G\\
R2: & k_2*M\\
R3: & k_3*M\\
R4: & k_4*P
\end{pmatrix} 
=\left(
{\begin{array}{c}
{\frac  {dG}{dt}=  0}\\[6pt]
{\frac  {dM}{dt} = k_1*G-k_3*M}\\[6pt]
{\frac  {dP}{dt} = k_2*M-k_4*P}\\[6pt] 
\end{array}}
\right)\]

\

\clearpage

\

Gene regulation

\[{\dot  {y}} 
 = \Gamma *V 
 =  \begin{pmatrix}
 & R1 & R2 & R3\\
S &  -1 & +1 & 0\\
E &  -1 & +1 & +1\\
SE &  +1 & -1 & -1\\
P &  0 & 0 & +1
\end{pmatrix} * 
\begin{pmatrix}
R1: & k_1*E*S\\
R2: & k_2*ES\\
R3: & k_3*ES
\end{pmatrix} 
=\left(
{\begin{array}{c}
{\frac  {dS}{dt}=  -k_1*E*S + k_2*ES}\\[6pt]
{\frac  {dE}{dt} = -k_1*E*S + (k_2+k_3)*ES}\\[6pt]
{\frac  {dES}{dt} =  k_1*E*S - (k_2+k_3)*ES}\\[6pt]
{\frac  {dP}{dt} = k_3*ES}\\[6pt] 
\end{array}}
\right)\]

\end{document}





